\documentclass{article}
\title{Show Integral}
\author{Vivian Duong}
\usepackage{amssymb}
\usepackage{amsmath}
\usepackage{amsthm}
\usepackage[pdftex]{hyperref}
\newtheorem{definition}{Definition}

\begin{document}

Show that 

\begin{equation}
\int_0^\infty e^{-x^2} \mathrm{d}x = \dfrac{\sqrt{\pi}}{2}
\end{equation}
Let

\begin{center}
$\mathrm{I} = \int_0^\infty e^{-x^2} \mathrm{d}x$
\\

$\mathrm{I^2} = \int_0^\infty e^{-x^2} \mathrm{d}x[\int_0^\infty e^{-y^2} \mathrm{d}y]$
\\

$\mathrm{I^2} = \int_0^\infty e^{-x^2} e^{-y^2}  \mathrm{d}x \mathrm{d}y$
\\

\begin{flushright}
$r = \sqrt{x^2 + y^2}$
\end{flushright}


$\mathrm{I^2} = \int_0^\infty \int_0^\infty e^{-x^2 - y^2}  \mathrm{d}x \mathrm{d}y$
\\

$\mathrm{I^2} = \int_0^\infty \int_0^{\frac{\pi}{2}} e^{-r^2} r\mathrm{d}\theta \mathrm{d}r$
\\

$\mathrm{I^2} = \dfrac{\pi}{2}\int_0^\infty e^{-r^2} r\mathrm{d}r$
\begin{flushright}
$u = -r^2$

$\mathrm{d}u = -2r\mathrm{d}r$

$\dfrac{\mathrm{d}u}{-2} = r\mathrm{d}r$
\end{flushright}

$\mathrm{I^2} = \dfrac{\pi}{-4}\int_0^\infty e^{u} \mathrm{d}u$
\\

$\mathrm{I^2} = \dfrac{\pi}{-4}[e^{-r^2}|_0^\infty]$
\\

$\mathrm{I^2} = \dfrac{\pi}{-4}[\lim_{r \rightarrow \infty} e^{-r^2} - 1]$
\\

$\mathrm{I^2} = \dfrac{\pi}{-4}[0 - 1]$
\\

$\mathrm{I^2} = \dfrac{\pi}{4}$
\\

$\sqrt{\mathrm{I^2}} = \sqrt{\dfrac{\pi}{4}}$
\\

$\mathrm{I} = \dfrac{\pi}{2}$
\\

$\int_0^\infty e^{-x^2} \mathrm{d}x = \dfrac{\pi}{2}$

\end{center}

\end{document}
