\documentclass{article}
\title{2 Proofs that the Derivative of x to the nth power equals nx to the n-1 power}
\author{Vivian Duong}
\date{}
\usepackage{enumerate}
\usepackage{amssymb}
\usepackage{amsmath}
\usepackage{fullpage}
\usepackage{amsthm}
\usepackage[pdftex]{hyperref}
\usepackage{soul}
\usepackage{ulem}
\newtheorem{definition}{Definition}

\begin{document}
\maketitle
Two proofs that
$\dfrac{\mathrm{d}}{\mathrm{d}x} x^n = nx^{n-1}$


\begin{proof}
\begin{center}
Here is the first one. 
\newline 
Let $ y = x^n$

$ln(y) = ln(x^n)$

$ln(y) = nln(x)$

$\dfrac{\mathrm{d}}{\mathrm{d}x}[ln(y(x))] = \dfrac{\mathrm{d}}{\mathrm{d}x}[nln(x)]$


$\dfrac{\mathrm{d}x}{\mathrm{d}y}.\dfrac{\mathrm{d}y}{\mathrm{d}x} = n \dfrac{1}{x}$

$\dfrac{1}{y}.\dfrac{\mathrm{d}y}{\mathrm{d}x} = n \dfrac{1}{x}$

$\dfrac{\mathrm{d}y}{\mathrm{d}x} = \dfrac{yn}{x}$

$\dfrac{\mathrm{d}}{\mathrm{d}x}y = \dfrac{nx^n}{x}$

$\dfrac{\mathrm{d}}{\mathrm{d}x}(x^n) = nx^{n-1}$

\end{center}
\end{proof}

Here is a another way.

\begin{proof}
\begin{center}
Let $f(x) = x^n$
\newline
$f'(a) = \lim_{x \rightarrow a} \dfrac{f(x)-f(a)}{x-a}$
\newline
$ =  \lim_{x \rightarrow a} \dfrac{x^n-a^n}{x-a}$

$ = \lim_{x \rightarrow a} \dfrac{\sout{(x-a)}(x^{n-1}+ax^{n-2} + a^2x^{n-3} +... + a^{n-3}x^2 + a^{n-2}x + a^{n-1}}{\sout{x-a}}$

$ = \lim_{x \rightarrow a} x^{n-1}+ax^{n-2} + a^2x^{n-3} +... + a^{n-3}x^2 + a^{n-2}x + a^{n-1}$

$ = \lim_{x \rightarrow a} a^{n-1}+aa^{n-2} + a^2a^{n-3} +... + a^{n-3}a^2 + a^{n-2}a + a^{n-1}$

$ = \lim_{x \rightarrow a} a^{n-1}+a^{n-1} + a^{n-1} +... + a^{n-1} + a^{n-1} + a^{n-1}$

$f'(a) = na^{n-1}$

$f'(x) = nx^{n-1}$

\end{center}
\end{proof}


\end{document}

